clean up fir-contract example a little

example/Fir.CheckN.fst
@@ -1,4 +1,4 @@
-(* This is an example of proving interesting things by mixing induction over lists with proofs about streams. *)
+(* This is an example of proving semi-interesting things by mixing induction over lists with proofs about streams. *)
 module Fir.CheckN
 
 open Pipit.Sugar.Vanilla
@@ -14,15 +14,16 @@ module R = FStar.Real
 
 let treal = Pipit.Prim.Vanilla.TReal
 
-type fir_contract (mul: R.real) =
-  Check.contract table [treal] treal
-    (Check.exp_of_stream1 (fun i -> (const (R.of_int (-1))) <=^ i /\ i <=^ r1))
-    (Check.exp_of_stream2 (fun r i -> r <=^ const mul))
+let bibo_rely = Check.exp_of_stream1 #_ #treal
+  (fun i -> (const (R.of_int (-1))) <=^ i /\ i <=^ r1)
 
-// type fir_contract' (mul: list R.real) =
-//   Check.contract1 table [treal] treal
-//     (fun i -> abs i <=^ r1)
-//     (fun i r -> abs r <=^ const mul)
+let bibo_guar (mul: R.real) = Check.exp_of_stream2 #_ #treal #treal
+  (fun r i -> r <=^ const mul)
+
+type bibo_contract (mul: R.real) =
+  Check.contract table [treal] treal
+    bibo_rely
+    (bibo_guar mul)
 
 let r_abs (r: R.real): R.real =
   R.(if r >=. zero then r else (zero -. r))
@@ -34,20 +35,18 @@ let rec sum_abs (coeffs: list R.real) =
 
 #push-options "--split_queries always"
 
-
-#push-options "--print_full_names"
-let rec fir_body (coeffs: list R.real):
-  fir_contract (sum_abs coeffs) =
-  let r = (Check.exp_of_stream1 (fun i -> (const (R.of_int (-1))) <=^ i /\ i <=^ r1)) in
-  let g = (Check.exp_of_stream2 (fun r i -> r <=^ const (sum_abs coeffs))) in
+let rec fir (coeffs: list R.real):
+  bibo_contract (sum_abs coeffs) =
   match coeffs with
   | [] ->
-    let e = Check.exp_of_stream1 (fun _ -> zero) in
-    assert (Check.contract_system_induct_k1' r g e) by (T.norm_full ["Fir"]);
-    Check.contract_of_exp1 r g e
+    let ret = Check.exp_of_stream1 (fun _ -> const 0.0R) in
+
+    assert (Check.contract_system_induct_k1' bibo_rely (bibo_guar 0.0R) ret) by (T.norm_full ["Fir"]);
+    Check.contract_of_exp1 _ _ ret
   | c :: coeffs' ->
-    let e = Check.exp_of_stream1 (fun input ->
-      let fir' = Check.stream_of_contract1 (fir_body coeffs') (fby 0.0R input) in
-      (input *^ const c) +^ fir') in
-    assert (Check.contract_system_induct_k1' r g e) by (T.norm_full ["Fir"]; T.dump "X");
-    Check.contract_of_exp1 r g e
+    let fir': bibo_contract (sum_abs coeffs') = fir coeffs' in
+    let ret = Check.exp_of_stream1 (fun input ->
+      (input *^ const c) +^ Check.stream_of_contract1 fir' (fby 0.0R input)) in
+
+    assert (Check.contract_system_induct_k1' bibo_rely (bibo_guar (sum_abs coeffs)) ret) by (T.norm_full ["Fir"]);
+    Check.contract_of_exp1 _ _ ret
